new/golang/defn/predeclared.v
@@ -479,8 +479,8 @@ Class PredeclaredSemantics `{!GoSemanticsFunctions} :=
   #[global] go_eq_bool :: go.AlwaysSafelyComparable go.bool Datatypes.bool;
   #[global] underlying_bool :: go.bool ↓u go.bool;
   #[global] type_repr_bool :: go.TypeRepr go.bool Datatypes.bool;
-  #[global] convert_untyped_bool `{!to ↓u go.bool} (b : Datatypes.bool) ::
-    go.GoExprEq (Convert go.untyped_bool to #b) #b;
+  #[global] convert_untyped_bool (b : Datatypes.bool) ::
+    go.ConvertUnderlying go.untyped_bool go.bool #b #b;
 
   #[global] untyped_int_semantics :: UntypedIntSemantics;
   #[global] int_semantics :: IntSemantics;
@@ -499,8 +499,8 @@ Class PredeclaredSemantics `{!GoSemanticsFunctions} :=
   #[global] underlying_string :: go.string ↓u go.string;
   #[global] plus_string (v1 v2 : go_string) :: go.IsGoOp GoPlus go.string (#v1, #v2) #(v1 ++ v2);
   #[global] type_repr_string :: go.TypeRepr go.string go_string;
-  #[global] convert_untyped_string `{!to ↓u go.string} (s : go_string) ::
-    go.GoExprEq (Convert go.untyped_string to #s) #s;
+  #[global] convert_untyped_string (s : go_string) ::
+    go.ConvertUnderlying go.untyped_string go.string #s #s;
 
   #[global] underlying_untyped_nil :: go.untyped_nil ↓u go.untyped_nil;
   #[global] convert_nil_pointer elem ::
