new/golang/theory/map.v
@@ -3,27 +3,19 @@ From New.golang.theory Require Export mem array predeclared auto.
 
 Set Default Proof Using "Type".
 
-Section safe_map_key.
-Context {ext : ffi_syntax} {go_gctx : GoGlobalContext} {go_lctx : GoLocalContext}
-  {sem_fn : GoSemanticsFunctions} {pre_sem : go.PreSemantics}.
-Local Set Default Proof Using "All".
-Class SafeMapKey {K} key_type (k : K) :=
-  {
-    safe_map_go_eq :
-      ∃ (b : bool), go.GoExprEq (go_eq key_type #k #k) (#b);
-  }.
-
-Global Instance safe_map_key_is_go_eq {K} key_type (k : K) (b : bool) :
-  go.GoExprEq (go_eq key_type #k #k) #b → SafeMapKey key_type k.
-Proof.
-  intros ?. constructor. by eexists.
-Qed.
-End safe_map_key.
-
 Section defns_and_lemmas.
 Context `{ffi_sem: ffi_semantics} `{!ffi_interp ffi} `{!heapGS Σ}
   {sem_fn : GoSemanticsFunctions} {pre_sem : go.PreSemantics}.
 Local Set Default Proof Using "All".
+
+Class SafeMapKey {K} key_type (k : K) :=
+  {
+    wp_go_eq_safe_map_key : ∀ stk E Φ, (∀ v, Φ v) -∗ WP (go_eq key_type #k #k) @ stk; E {{ Φ }};
+  }.
+
+Global Instance safe_map_key_is_go_eq {K} key_type (k : K) (b : bool) :
+  go.GoExprEq (go_eq key_type #k #k) #b → SafeMapKey key_type k.
+Proof. intros ?. constructor. iIntros. wp_auto. done. Qed.
 
 (* TODO: reading from nil map. Want to say that an owned map is not nil, which
    requires knowing that wp_ref gives non-null pointers. *)
@@ -83,28 +75,13 @@ Proof. rewrite own_map_unseal. apply _. Qed.
 Notation "mref ↦$ dq m" := (own_map mref dq m)
                             (at level 20, dq custom dfrac at level 50, format "mref  ↦$ dq  m").
 
-Local Instance safe_key_check (k : K) (v : val) `{!go.GoExprEq (go_eq key_type #k #k) v} :
-  PureWp True (Convert key_type go.any (# k) =⟨go.any⟩ Convert key_type go.any (# k)) v.
-Proof.
-  pure_wp_start. pose proof underlying_trivial key_type.
-  wp_auto_lc 1. destruct go.is_interface_type eqn:Hi.
-    - destruct (underlying key_type); try done.
-      rewrite (go.go_eq_interface_eq _ l).
-      assert (go.GoExprEq (go_eq (go.InterfaceType l) #k #k) v).
-      { unshelve eapply go.go_eq_underlying.
-        constructor. rewrite go.is_underlying go.is_underlying //. }
-      wp_auto. wp_end.
-    - wp_auto. rewrite decide_True //. wp_auto. wp_end.
-Qed.
-
 Lemma wp_map_insert key_type l (m : gmap K V) k v {Hsafe : SafeMapKey key_type k} :
   {{{ l ↦$ m }}}
     map.insert key_type #l #k #v
   {{{ RET #(); l ↦$ <[k := v]> m }}}.
 Proof.
-  destruct Hsafe as [[? Hsafe]].
   rewrite own_map_unseal.
-  iIntros (?) "Hm HΦ". iNamed "Hm". wp_call.
+  iIntros (?) "Hm HΦ". iNamed "Hm". wp_call. wp_apply wp_go_eq_safe_map_key as "%".
   wp_apply (_internal_wp_untyped_read with "Hown"). iIntros "Hown".
   wp_auto.
   wp_apply (_internal_wp_untyped_store with "Hown"). iIntros "Hown".
@@ -124,8 +101,8 @@ Lemma wp_map_delete l (m : gmap K V) k key_type elem_type {Hsafe : SafeMapKey ke
         #l #k
   {{{ RET #(); l ↦$ delete k m }}}.
 Proof.
-  destruct Hsafe as [[? Hsafe]].
   wp_start as "Hm". rewrite own_map_unseal. iNamed "Hm".
+  wp_apply wp_go_eq_safe_map_key as "%".
   wp_apply (_internal_wp_untyped_read with "Hown") as "Hown".
   wp_apply (_internal_wp_untyped_store with "Hown") as "Hown".
   iApply "HΦ". iFrame "Hown".
@@ -143,10 +120,10 @@ Lemma wp_map_lookup2 key_type elem_type mref (m : gmap K V) k dq {Hsafe : SafeMa
     map.lookup2 key_type elem_type #mref #k
   {{{ RET (#(default (zero_val V) (m !! k)), #(bool_decide (is_Some (m !! k)))); mref ↦${dq} m }}}.
 Proof.
-  destruct Hsafe as [[? Hsafe]].
   wp_start as "Hm".
   rewrite own_map_unseal. iNamed "Hm".
   iDestruct (heap_pointsto_non_null with "Hown") as "%H".
+  wp_apply wp_go_eq_safe_map_key as "%".
   wp_if_destruct; first by exfalso.
   wp_apply (_internal_wp_untyped_read with "Hown") as "Hown".
   erewrite go.map_lookup_pure; last done.
@@ -160,8 +137,7 @@ Global Instance pure_wp_map_nil_lookup2 key_type elem_type (k : K)
   {Hsafe : SafeMapKey key_type k} :
   PureWp True (map.lookup2 key_type elem_type #map.nil #k) (#(zero_val V), #false)%V.
 Proof.
-  destruct Hsafe as [[? Hsafe]].
-  pure_wp_start. wp_end.
+  pure_wp_start. wp_apply wp_go_eq_safe_map_key as "%". wp_end.
 Qed.
 
 Lemma wp_map_lookup1 key_type elem_type mref (m : gmap K V) k dq {Hsafe : SafeMapKey key_type k} :
